LeanMachines/Event/Algebra/Convergent.lean
@@ -10,12 +10,6 @@ import LeanMachines.Event.Algebra.Ordinary
 import LeanMachines.Event.Algebra.Basic
 
 
-
-
-
-
-
-
 /-!
 ## Algebraic properties of events
 
@@ -25,7 +19,7 @@ and convergent events (experimental, not documented).
 -/
 
 @[simp]
-def mapAnticipatedEvent [Preorder v] [Machine CTX M] (f : α → β) (ev : _AnticipatedEvent v M γ α) : _AnticipatedEvent v M γ β :=
+def mapAnticipatedEvent [Preorder v] [Machine CTX M] (f : α → β) (ev : AnticipatedEvent v M γ α) : AnticipatedEvent v M γ β :=
   {
     guard := ev.guard
     action := fun m x grd => let (y, m') := ev.action m x grd
@@ -35,15 +29,15 @@ def mapAnticipatedEvent [Preorder v] [Machine CTX M] (f : α → β) (ev : _Anti
     nonIncreasing := ev.nonIncreasing
   }
 
-instance [Preorder v] [Machine CTX M] : Functor (_AnticipatedEvent v M γ) where
+instance [Preorder v] [Machine CTX M] : Functor (AnticipatedEvent v M γ) where
   map := mapAnticipatedEvent
 
-instance [Preorder v] [Machine CTX M] : LawfulFunctor (_AnticipatedEvent v M γ) where
-  map_const := rfl
+instance [Preorder v] [Machine CTX M] : LawfulFunctor (AnticipatedEvent v M γ) where
+  map_const := by intros ; rfl
   id_map := by intros ; rfl
   comp_map := by intros ; rfl
 
-def mapConvergentEvent [Preorder v] [WellFoundedLT v] [Machine CTX M] (f : α → β) (ev : _ConvergentEvent v M γ α) : _ConvergentEvent v M γ β :=
+def mapConvergentEvent [Preorder v] [WellFoundedLT v] [Machine CTX M] (f : α → β) (ev : ConvergentEvent v M γ α) : ConvergentEvent v M γ β :=
   {
     guard := ev.guard
     action := fun m x grd => let (y, m') := ev.action m x grd
@@ -53,10 +47,10 @@ def mapConvergentEvent [Preorder v] [WellFoundedLT v] [Machine CTX M] (f : α �
     convergence := ev.convergence
   }
 
-instance [Preorder v] [WellFoundedLT v] [Machine CTX M] : Functor (_ConvergentEvent v M γ) where
+instance [Preorder v] [WellFoundedLT v] [Machine CTX M] : Functor (ConvergentEvent v M γ) where
   map := mapConvergentEvent
 
-instance [Preorder v] [WellFoundedLT v] [Machine CTX M] : LawfulFunctor (_ConvergentEvent v M γ) where
+instance [Preorder v] [WellFoundedLT v] [Machine CTX M] : LawfulFunctor (ConvergentEvent v M γ) where
   map_const := rfl
   id_map := by intros ; rfl
   comp_map := by intros ; rfl
@@ -64,13 +58,13 @@ instance [Preorder v] [WellFoundedLT v] [Machine CTX M] : LawfulFunctor (_Conver
 /- Contravariant functor -/
 
 abbrev CoAnticipatedEvent (v) [Preorder v] (M) [Machine CTX M] (α) (β) :=
-   _AnticipatedEvent v M β α
+   AnticipatedEvent v M β α
 
 @[simp]
-def AnticipatedEvent_from_CoAnticipatedEvent [Preorder v] [Machine CTX M] (ev : CoAnticipatedEvent v M α β) : _AnticipatedEvent v M β α := ev
+def AnticipatedEvent_from_CoAnticipatedEvent [Preorder v] [Machine CTX M] (ev : CoAnticipatedEvent v M α β) : AnticipatedEvent v M β α := ev
 
 @[simp]
-def CoAnticipatedEvent_from_AnticipatedEvent [Preorder v] [Machine CTX M] (ev : _AnticipatedEvent v M α β) : CoAnticipatedEvent v M β α := ev
+def CoAnticipatedEvent_from_AnticipatedEvent [Preorder v] [Machine CTX M] (ev : AnticipatedEvent v M α β) : CoAnticipatedEvent v M β α := ev
 
 instance [Preorder v] [Machine CTX M]: ContravariantFunctor (CoAnticipatedEvent v M γ) where
   contramap {α β} (f : β → α) (ev : CoAnticipatedEvent v M γ α) :=
@@ -97,13 +91,13 @@ instance [Preorder v] [Machine CTX M] : LawfullContravariantFunctor (CoAnticipat
   cmap_comp _ _ := by rfl
 
 abbrev CoConvergentEvent (v) [Preorder v] [WellFoundedLT v] (M) [Machine CTX M] (α) (β) :=
-   _ConvergentEvent v M β α
+   ConvergentEvent v M β α
 
 @[simp]
-def ConvergentEvent_from_CoConvergentEvent [Preorder v] [WellFoundedLT v] [Machine CTX M] (ev : CoConvergentEvent v M α β) : _ConvergentEvent v M β α := ev
+def ConvergentEvent_from_CoConvergentEvent [Preorder v] [WellFoundedLT v] [Machine CTX M] (ev : CoConvergentEvent v M α β) : ConvergentEvent v M β α := ev
 
 @[simp]
-def CoConvergentEvent_from_ConvergentEvent [Preorder v] [WellFoundedLT v] [Machine CTX M] (ev : _ConvergentEvent v M α β) : CoConvergentEvent v M β α := ev
+def CoConvergentEvent_from_ConvergentEvent [Preorder v] [WellFoundedLT v] [Machine CTX M] (ev : ConvergentEvent v M α β) : CoConvergentEvent v M β α := ev
 
 instance [Preorder v] [WellFoundedLT v] [Machine CTX M]: ContravariantFunctor (CoConvergentEvent v M γ) where
   contramap {α β} (f : β → α) (ev : CoConvergentEvent v M γ α) :=
@@ -133,8 +127,8 @@ instance [Preorder v] [WellFoundedLT v] [Machine CTX M] : LawfullContravariantFu
 
 /- Profunctor -/
 
-instance [Preorder v] [Machine CTX M] : Profunctor (_AnticipatedEvent v M) where
-  dimap {α β} {γ δ} (f : β → α) (g : γ → δ) (ev : _AnticipatedEvent v M α γ) : _AnticipatedEvent v M β δ :=
+instance [Preorder v] [Machine CTX M] : Profunctor (AnticipatedEvent v M) where
+  dimap {α β} {γ δ} (f : β → α) (g : γ → δ) (ev : AnticipatedEvent v M α γ) : AnticipatedEvent v M β δ :=
     let event := Profunctor.dimap f g ev.toEvent
     {
       guard := fun m x => ev.guard m (f x)
@@ -162,12 +156,12 @@ instance [Preorder v] [Machine CTX M] : Profunctor (_AnticipatedEvent v M) where
 
     }
 
-instance [Preorder v] [Machine CTX M] : LawfulProfunctor (_AnticipatedEvent v M) where
+instance [Preorder v] [Machine CTX M] : LawfulProfunctor (AnticipatedEvent v M) where
   dimap_id := rfl
   dimap_comp _ _ _ _ := rfl
 
-instance [Preorder v] [Machine CTX M] : StrongProfunctor (_AnticipatedEvent v M) where
-  first' {α β γ} (ev : _AnticipatedEvent v M α β): _AnticipatedEvent v M (α × γ) (β × γ) :=
+instance [Preorder v] [Machine CTX M] : StrongProfunctor (AnticipatedEvent v M) where
+  first' {α β γ} (ev : AnticipatedEvent v M α β): AnticipatedEvent v M (α × γ) (β × γ) :=
     let event := StrongProfunctor.first' ev.toEvent
     {
       guard := fun m (x, y) => ev.guard m x ∧ event.guard m (x, y)
@@ -184,11 +178,11 @@ instance [Preorder v] [Machine CTX M] : StrongProfunctor (_AnticipatedEvent v M)
 
     }
 
-instance [Preorder v] [Machine CTX M] : LawfulStrongProfunctor (_AnticipatedEvent v M) where
+instance [Preorder v] [Machine CTX M] : LawfulStrongProfunctor (AnticipatedEvent v M) where
   -- XXX : at some point the laws should be demonstrated
 
-instance [Preorder v] [WellFoundedLT v] [Machine CTX M] : Profunctor (_ConvergentEvent v M) where
-  dimap {α β} {γ δ} (f : β → α) (g : γ → δ) (ev : _ConvergentEvent v M α γ) : _ConvergentEvent v M β δ :=
+instance [Preorder v] [WellFoundedLT v] [Machine CTX M] : Profunctor (ConvergentEvent v M) where
+  dimap {α β} {γ δ} (f : β → α) (g : γ → δ) (ev : ConvergentEvent v M α γ) : ConvergentEvent v M β δ :=
     let event := Profunctor.dimap f g ev.toEvent
     {
       guard := fun m x => ev.guard m (f x)
@@ -215,12 +209,12 @@ instance [Preorder v] [WellFoundedLT v] [Machine CTX M] : Profunctor (_Convergen
         apply Hni
     }
 
-instance [Preorder v] [WellFoundedLT v] [Machine CTX M] : LawfulProfunctor (_ConvergentEvent v M) where
+instance [Preorder v] [WellFoundedLT v] [Machine CTX M] : LawfulProfunctor (ConvergentEvent v M) where
   dimap_id := rfl
   dimap_comp _ _ _ _ := rfl
 
-instance [Preorder v] [WellFoundedLT v] [Machine CTX M] : StrongProfunctor (_ConvergentEvent v M) where
-  first' {α β γ} (ev : _ConvergentEvent v M α β): _ConvergentEvent v M (α × γ) (β × γ) :=
+instance [Preorder v] [WellFoundedLT v] [Machine CTX M] : StrongProfunctor (ConvergentEvent v M) where
+  first' {α β γ} (ev : ConvergentEvent v M α β): ConvergentEvent v M (α × γ) (β × γ) :=
     let event := StrongProfunctor.first' ev.toEvent
     {
       guard := fun m (x, y) => ev.guard m x ∧ event.guard m (x, y)
@@ -237,7 +231,7 @@ instance [Preorder v] [WellFoundedLT v] [Machine CTX M] : StrongProfunctor (_Con
         apply ev.convergence m x Hinv
     }
 
-instance [Preorder v] [WellFoundedLT v] [Machine CTX M] : LawfulStrongProfunctor (_ConvergentEvent v M) where
+instance [Preorder v] [WellFoundedLT v] [Machine CTX M] : LawfulStrongProfunctor (ConvergentEvent v M) where
   -- XXX : at some point the laws should be demonstrated
 
 /-
