LeanMachines/Examples/Buffer/Buffer0.lean
@@ -1,0 +1,116 @@
+import Mathlib.Tactic
+
+import LeanMachines.Event.Basic
+import LeanMachines.Event.Ordinary
+--import LeanMachines.Event.Convergent
+
+--import LeanMachines.NonDet.Ordinary
+--import LeanMachines.NonDet.Convergent
+
+/-!
+# The Buffer example
+
+This is a very simple example specification of a bounded buffer, developed in
+three refinement steps:
+
+ 1. An abstract machine `Buffer0` (this file), only tracking the number of buffered elements
+
+ 2. A more concrete machine `Buffer1` (file `Buffer1.lean`), which actually buffers elements
+  in a list, managed in a non-deterministic way
+
+ 3. A functional (deterministic) machine `Buffer2` (file `Buffer2.lean`) that uses a list representation
+  and puts/retrieves elements using a priority-scheme
+
+The proof obligations are rather trivial, except for the last step since priorities "break"
+the structural induction principle of lists.
+
+This is the running illustrative example of the IFM2024 paper:
+
+    Stateful Functional Modeling with Refinement (a Lean4 framework)
+
+-/
+
+/-!
+
+## Abstract machine
+
+At the most abstract level, only the number of elements in the buffer is tracked.
+
+-/
+
+namespace Buffer
+
+/-- The (shared) context for all the machines -/
+structure BufContext where
+  /-- The maximum size of the buffer -/
+  maxSize : Nat
+  maxSizeProp : maxSize > 0
+
+/-- The state of the abstract machine -/
+structure B0 (ctx : BufContext) where
+  /-- The current size of the buffer -/
+  size : Nat
+
+/-- The instantiation of the machine -/
+instance: Machine BufContext (B0 ctx) where
+  context := ctx
+  invariant b0 := b0.size ≤ ctx.maxSize
+
+/-- Initialization event (no parameter, empty buffer)-/
+def B0.Init : _InitEvent (B0 ctx) Unit Unit :=
+  newInitEvent'' {
+    init _ := { size := 0 }
+    safety := fun _ => by simp [Machine.invariant]
+  }
+
+/-- Event: adding an element to the buffer (no parameter,
+since we only track the number of elements)-/
+def B0.Put : OrdinaryEvent (B0 ctx) Unit Unit :=
+  newEvent'' {
+    guard := fun b0 => b0.size < ctx.maxSize
+    action := fun b0 _ => { size := b0.size + 1 }
+    safety := fun b0 => by exact fun _ Hgrd => Hgrd
+  }
+
+/-- Event : fetching (retrieving) an element.
+At the abstract level, this meanins just decrementing the size.
+The Event is proved convergent.
+-/
+def B0.Fetch : ConvergentEvent Nat (B0 ctx) Unit Unit :=
+  newConvergentEvent'' {
+    guard := fun b0 => b0.size > 0
+    action := fun b0 _ => { size := b0.size - 1 }
+    safety := fun b0 => by
+      simp [Machine.invariant]
+      intros H _
+      exact Nat.le_add_right_of_le H
+
+    variant := fun b0 => b0.size
+    convergence := fun b0 => by
+      simp [Machine.invariant]
+  }
+
+/-- Event : querying the current size of the buffer. -/
+def B0.GetSize : OrdinaryEvent (B0 ctx) Unit Nat :=
+  newEvent {
+    action := fun b0 () _ => (b0.size, b0)
+    safety := fun b0 () => by simp
+  }
+
+/-- Event : inserting an unspecified number of elements
+ (non-deterministic event) -/
+def B0.Batch : OrdinaryNDEvent (B0 ctx) Unit Unit :=
+  newNDEvent'' {
+    guard := fun b0 => b0.size < ctx.maxSize
+    effect := fun b0 _ b0'  => ∃ n > 0, b0'.size = b0.size + n ∧ b0'.size ≤ ctx.maxSize
+
+    feasibility := fun b0 => by
+      simp [Machine.invariant]
+      intros _ Hgrd
+      exists { size := b0.size + 1 }
+      exists 1
+
+    safety := fun b0 => by simp [Machine.invariant]
+  }
+
+end Buffer
